refactor: reparametrize by concrete CFG and remove validCFG

Flow/Analysis/WorklistProofs.lean
@@ -328,11 +328,11 @@ namespace Flow.Analysis
 open Flow.Analysis Flow.Analysis.Generic
 
 variable {Node Edge State : Type} [DecidableEq Node] [DecidableEq Edge]
-variable [ls : LangSem Node Edge State]
+variable {g : AnalysisCFG Node Edge}
+variable [ls : LangSem Node Edge State g]
 
 theorem postFixpoint_of_isForwardPostFixpoint
     [Bot A] [Max A] [FiniteHeight A] [ll : LatticeLike A]
-    {g : AnalysisCFG Node Edge}
     (nodeTransfer : Node -> A -> A) (edgeTransfer : Edge -> A -> A)
     [tm : TransferMono nodeTransfer edgeTransfer]
     (entryInit : A) (outF : StateN g A)
@@ -341,7 +341,7 @@ theorem postFixpoint_of_isForwardPostFixpoint
       ({ L := A
        , nodeTransfer := nodeTransfer
        , edgeTransfer := edgeTransfer
-       , entry := entryInit } : DFA Node Edge State)
+       , entry := entryInit } : DFA Node Edge State g)
       (fun n =>
         if h : n ∈ g.nodes then
           expectedIn g edgeTransfer entryInit outF ⟨n, h⟩
@@ -385,16 +385,16 @@ open Flow.Analysis Flow.Analysis.Generic
 
 /-- Analysis bundle instance -/
 structure Analysis (Node Edge State : Type)
-    [DecidableEq Node] [DecidableEq Edge] [ls : LangSem Node Edge State] where
-  dfa : DFA Node Edge State
-  g : AnalysisCFG Node Edge
-  gValid : ls.ValidCFG g
+    [DecidableEq Node] [DecidableEq Edge]
+    {g : AnalysisCFG Node Edge}
+    [ls : LangSem Node Edge State g] where
+  dfa : DFA Node Edge State g
   botL : Bot dfa.L
   maxL : Max dfa.L
   decEqL : DecidableEq dfa.L
   fhL : FiniteHeight dfa.L
   llL : LatticeLike dfa.L
-  semantics : DFASemantics g gValid dfa
+  semantics : DFASemantics g dfa
   mono_absorb :
     ∀ {ℓ ℓ' : dfa.L} {σ : State},
       ℓ ⊑ ℓ' -> semantics.Corr ℓ σ -> semantics.Corr ℓ' σ
@@ -402,17 +402,21 @@ structure Analysis (Node Edge State : Type)
       TransferMono dfa.nodeTransfer dfa.edgeTransfer
 
 structure AnalysisResult {Node Edge State : Type}
-    [DecidableEq Node] [DecidableEq Edge] [ls : LangSem Node Edge State]
-    (a : Analysis Node Edge State) (g : AnalysisCFG Node Edge) (gValid : ls.ValidCFG g) where
+    [DecidableEq Node] [DecidableEq Edge]
+    {g : AnalysisCFG Node Edge}
+    [ls : LangSem Node Edge State g]
+    (a : Analysis (ls := ls) Node Edge State) where
   inFacts : Node -> a.dfa.L
   outFacts : Node -> a.dfa.L
   isPostFix : letI := a.maxL; Generic.PostFixpoint g a.dfa inFacts
   inFacts_entry : letI := a.maxL; a.dfa.entry ⊑ (inFacts g.entry)
 
 def analyze {Node Edge State : Type}
-    [DecidableEq Node] [DecidableEq Edge] [ls : LangSem Node Edge State]
-    (a : Analysis Node Edge State) (g : AnalysisCFG Node Edge) (gValid : ls.ValidCFG g) :
-    AnalysisResult a g gValid :=
+    [DecidableEq Node] [DecidableEq Edge]
+    {g : AnalysisCFG Node Edge}
+    [ls : LangSem Node Edge State g]
+    (a : Analysis Node Edge State) :
+    AnalysisResult (ls := ls) a :=
   letI := a.botL
   letI := a.maxL
   letI := a.decEqL
